  

\begin{center}
\begin{pseudocode}[doublebox]{PNUFGT}{N, \delta}
\label{alg:pnufgt}
\COMMENT{Computes $y = S x$} \\
\mbox{Send $x$ from $\widehat{L}$ to $\widehat{R}$} \\
\mbox{Compute $i^{(\widehat{L})} = K_{II}^{(\widehat{L})} x$} \\
\mbox{Compute $i^{(\widehat{R})} = K_{II}^{(\widehat{R})} x$} \\
\mbox{Compute $v_{\widehat{L}} = K_{\widehat{L}I} x$} \\
\mbox{Compute $v_{\widehat{R}} = K_{\widehat{R}I} x$} \\
\mbox{Solve $K_{\widehat{L}\widehat{L}} w_{\widehat{L}} = v_{\widehat{L}}$} \\
\mbox{Solve $K_{\widehat{R}\widehat{R}} w_{\widehat{R}} = v_{\widehat{R}}$} \\
\mbox{Compute $z^{(\widehat{L})} = K_{I\widehat{L}} w_{\widehat{L}}$} \\
\mbox{Compute $z^{(\widehat{R})} = K_{I\widehat{R}} w_{\widehat{R}}$} \\
\mbox{Compute $y^{(\widehat{L})} = i^{(\widehat{L})} - z^{(\widehat{L})}$} \\
\mbox{Compute $y^{(\widehat{R})} = i^{(\widehat{R})} - z^{(\widehat{R})}$} \\
\mbox{Send $y^{(\widehat{R})}$ from $\widehat{R}$ to $\widehat{L}$} \\
\mbox{Compute $y = y^{(\widehat{L})} + y^{(\widehat{R})}$} \\
\RETURN{y}
\end{pseudocode}
\end{center}